proof/TPOSR/Basic.v
@@ -11,7 +11,12 @@ Require Import Lambda.TPOSR.Env.
 Require Import Lambda.TPOSR.Types.
 Require Import Lambda.TPOSR.Thinning.
 Require Import Lambda.TPOSR.CtxReduction.
+Require Import Lambda.TPOSR.CtxExpansion.
+Require Import Lambda.TPOSR.CtxCoercion.
+Require Import Lambda.TPOSR.LeftReflexivity.
 Require Import Lambda.TPOSR.Substitution.
+Require Import Lambda.TPOSR.SubstitutionTPOSR.
+Require Import Lambda.TPOSR.RightReflexivity.
 
 Set Implicit Arguments.
 
