proof/TPOSR/RightReflexivity.v
@@ -3,10 +3,12 @@ Require Import Lambda.TPOSR.Reduction.
 Require Import Lambda.TPOSR.Conv.
 Require Import Lambda.TPOSR.LiftSubst.
 Require Import Lambda.TPOSR.Env.
-Require Import Lambda.TPOSR.Types.
+Require Import Lambda.TPOSR.TypesNoDerivs.
 Require Import Lambda.TPOSR.LeftReflexivity.
 Require Import Lambda.TPOSR.CtxReduction.
+Require Import Lambda.TPOSR.CtxCoercion.
 Require Import Lambda.TPOSR.Substitution.
+Require Import Lambda.TPOSR.SubstitutionTPOSR.
 
 Set Implicit Arguments.
 
@@ -14,13 +16,6 @@ Implicit Types i k m n p : nat.
 Implicit Type s : sort.
 Implicit Types A B M N T t u v : lterm.
 Implicit Types e f g : lenv.
-
-Lemma sub : forall g t u s, g |-- t ~= u : s -> t = u ->
-  forall e d d' T, g = T :: e -> e |-- d -> d' : T ->
-  e |-- lsubst d t ~= lsubst d' u : s.
-Proof.
-  induction 1 ; simpl ; intros ; try discriminate.
-  apply tposr_eq_tposr.
 
 Lemma ind_right_refl : 
   (forall e u v T, e |-- u -> v : T -> e |-- v -> v : T) /\
@@ -38,8 +33,9 @@ Proof.
   (P2:=fun e u v s => fun H : e |-- u >-> v : s =>
   e |-- u -> u : s /\ e |-- v -> v : s) ; simpl ; intros ; intuition ; auto with coc.
 
-  assert(red_in_env (A :: e) (A' :: e)) by eauto with coc.
+  assert(red_in_env (A :: e) (A' :: e)) by eauto with coc ecoc.
   apply tposr_prod with s1 ; eauto with coc ecoc.
+  
 
   assert(red_in_env (A :: e) (A' :: e)) by eauto with coc.
   apply tposr_conv with (Prod_l A' B) s2 ; auto with coc.
@@ -51,114 +47,97 @@ Proof.
   eauto with coc.
   apply tposr_conv with (Prod_l A B) s2 ; auto with coc.
   apply tposr_coerce_prod with s1 ; eauto with coc ecoc.
-  
-
-  apply tposr_app with A A s1 s2 ; auto with coc.
-  apply tposr_abs with s1 B s2 ; auto with coc.
+  apply tposr_coerce_sym.
+  apply substitution_tposr_coerce with A ; auto with coc.
+  apply tposr_conv with (lsubst N' B) s2 ; auto with coc.
+  apply substitution_tposr_tposr with A ; auto with coc ecoc.
+  apply tposr_coerce_sym.
+  apply substitution_tposr_coerce with A ; auto with coc.
+  eauto with coc.
   
   apply tposr_conv with A s ; auto with coc.
 
-  apply tposr_sum with s1 s2 ; auto with coc.
+  (* Subset *)
+  assert(red_in_env (A :: e) (A' :: e)) by eauto with coc.
+  apply tposr_subset ; eauto with coc ecoc.
 
-  apply tposr_pair with s1 s2 s3 ; auto with coc.
+  (* Sum *)
+  assert(red_in_env (A :: e) (A' :: e)) by eauto with coc.
+  apply tposr_sum with s1 s2 ; eauto with coc ecoc.
 
+  (* Pair *)
+  assert(red_in_env (A :: e) (A' :: e)) by eauto with coc.
+  apply tposr_conv with (Sum_l A' B') s3 ; auto with coc.
+  apply tposr_pair with s1 s2 s3 ; auto with coc ecoc.
+  eauto with coc ecoc.
+  apply tposr_conv with A s1 ; eauto with coc ecoc.
+ apply tposr_conv with (lsubst u B) s2 ; auto with coc.
+ apply substitution_tposr_coerce with A ; eauto with coc ecoc.
+ 
+  apply tposr_coerce_sum with s1 s2 ; eauto with coc ecoc.
+  apply coerce_red_env with (A :: e) ; auto with coc.
+  eauto with coc.
+
+  (* Pi1_l *)
+  apply tposr_conv with A' s1 ; auto with coc.
   apply tposr_pi1 with s1 s2 s3 ; eauto with coc ecoc.
 
+  (* Pi2 *)
+  apply tposr_conv with (lsubst (Pi1_l (Sum_l A' B') t') B') s2 ; auto with coc.  
+  apply tposr_pi2 with s1 s2 s3 ; eauto with coc ecoc.
+  apply tposr_coerce_sym.
+  apply substitution_tposr_coerce with A' ; eauto with coc.
+  apply coerce_coerce_env with (A :: e) ; eauto with coc.
   apply tposr_pi1 with s1 s2 s3 ; eauto with coc ecoc.
 
-  apply tposr_pi2 with s1 s2 s3 ; eauto with coc ecoc.
+  apply tposr_conv with  (lsubst u B) s2 ; auto with coc. 
+  apply tposr_coerce_sym.
+  apply substitution_tposr_coerce with A ; eauto with coc.
 
-  apply tposr_pi2 with s1 s2 s3 ; eauto with coc ecoc.
+  apply tposr_prod with s ; eauto with coc ecoc.
 
-  apply tposr_prod with s ; auto with coc.
+  apply tposr_prod with s ; eauto with coc ecoc.
 
-  apply tposr_prod with s ; auto with coc.
+  apply tposr_sum with s s' ; eauto with coc ecoc.
 
-  apply tposr_sum with s s' ; auto with coc.
-
-  apply tposr_sum with s s' ; auto with coc.
+  apply tposr_sum with s s' ; eauto with coc ecoc.
 Qed.
 
-Corollary refl_l : forall e u v T, e |-- u -> v : T -> e |-- u -> u : T.
-Proof (proj1 (ind_left_refl)).
+Corollary refl_r : forall e u v T, e |-- u -> v : T -> e |-- v -> v : T.
+Proof (proj1 (ind_right_refl)).
 
-Corollary tposrp_refl_l : forall e A B T, tposrp e A B T -> e |-- A -> A : T.
+Corollary tposrp_refl_r : forall e A B T, tposrp e A B T -> e |-- B -> B : T.
 Proof.
   induction 1 ; auto with coc.
-  apply (refl_l H).
+  apply (refl_r H).
 Qed.
 
 Corollary eq_refl_l : forall e u v s, e |-- u ~= v : s -> e |-- u -> u : s.
 Proof.
-  pose (proj1 (proj2 (proj2 (ind_left_refl)))).
+  pose (proj1 (proj2 (proj2 (ind_right_refl)))).
   intros.
   destruct (a _ _ _ _ H) ; auto.
 Qed. 
 
 Corollary eq_refl_r : forall e u v s, e |-- u ~= v : s -> e |-- v -> v : s.
 Proof.
-  pose (proj1 (proj2 (proj2 (ind_left_refl)))).
+  pose (proj1 (proj2 (proj2 (ind_right_refl)))).
   intros.
   destruct (a _ _ _ _ H) ; auto.
 Qed. 
 
 Corollary coerce_refl_l : forall e u v s, e |-- u >-> v : s -> e |-- u -> u : s.
 Proof.
-  pose (proj2 (proj2 (proj2 (ind_left_refl)))).
+  pose (proj2 (proj2 (proj2 (ind_right_refl)))).
   intros.
   destruct (a _ _ _ _ H) ; auto.
 Qed. 
 
 Corollary coerce_refl_r : forall e u v s, e |-- u >-> v : s -> e |-- v -> v : s.
 Proof.
-  pose (proj2 (proj2 (proj2 (ind_left_refl)))).
+  pose (proj2 (proj2 (proj2 (ind_right_refl)))).
   intros.
   destruct (a _ _ _ _ H) ; auto.
 Qed. 
 
-Hint Resolve refl_l tposrp_refl_l eq_refl_l eq_refl_r coerce_refl_l coerce_refl_r : coc.
-
-Lemma refl_r : forall e u v T, e |-- u -> v : T -> e |-- v -> v : T.
-Admitted.
-
-Corollary eq_refls : forall e u v s, e |-- u ~= v : s -> 
-  e |-- u -> u : Srt_l s /\ e |-- v -> v : Srt_l s.
-Admitted.
-
-Corollary coerce_refls : forall e u v s, e |-- u >-> v : s -> 
-  e |-- u -> u : Srt_l s /\ e |-- v -> v : Srt_l s.
-Admitted.
-
-Corollary eq_refl_l :  forall e u v s, e |-- u ~= v : s -> e |-- u -> u : Srt_l s.
-Proof.
-  intros.
-  apply (proj1 (eq_refls H)).
-Qed.
-
-Corollary eq_refl_r :  forall e u v s, e |-- u ~= v : s -> e |-- v -> v : Srt_l s.
-Proof.
-  intros.
-  apply (proj2 (eq_refls H)).
-Qed.
-
-Corollary coerce_refl_l :  forall e u v s, e |-- u >-> v : s -> e |-- u -> u : Srt_l s.
-Proof.
-  intros.
-  apply (proj1 (coerce_refls H)).
-Qed.
-
-Corollary coerce_refl_r :  forall e u v s, e |-- u >-> v : s -> e |-- v -> v : Srt_l s.
-Proof.
-  intros.
-  apply (proj2 (coerce_refls H)).
-Qed.
-
-Lemma tposrp_refl_r : forall e A B T, tposrp e A B T -> e |-- B -> B : T.
-Proof.
-  induction 1 ; auto with coc.
-  apply (refl_r H).
-Qed.
-
-Hint Resolve refl_r eq_refl_l eq_refl_r tposrp_refl_r : ecoc.
-Hint Resolve coerce_refl_r coerce_refl_l tposrp_refl_r : ecoc.
-
+Hint Resolve refl_r tposrp_refl_r eq_refl_l eq_refl_r coerce_refl_l coerce_refl_r : coc.
