proof/TPOSR/Thinning.v
@@ -94,6 +94,8 @@ apply wf_cons with (llift_rec 1 A0 n) s1 ; eauto with coc.
 
 assert (tposr_wf (llift_rec 1 A0 n :: f)) by (apply wf_cons with (llift_rec 1 A' n) s1 ; eauto with coc).
 apply tposr_pi1_red with (llift_rec 1 A' n) s1 (llift_rec 1 B' (S n))  s2 s3 (llift_rec 1 v' n); auto with coc.
+rewrite <- distr_llift_lsubst.
+auto with coc.
 
 assert (tposr_wf (llift_rec 1 A0 n :: f)) by (apply wf_cons with (llift_rec 1 A0 n) s1 ; eauto with coc).
 rewrite distr_llift_lsubst.
@@ -104,13 +106,14 @@ assert (tposr_wf (llift_rec 1 A0 n :: f)) by (apply wf_cons with (llift_rec 1 A'
 rewrite distr_llift_lsubst.
 simpl.
 apply tposr_pi2_red with (llift_rec 1 A' n) s1 (llift_rec 1 B' (S n))  s2 s3 (llift_rec 1 u' n); auto with coc.
+rewrite <- distr_llift_lsubst.
+auto with coc.
 
 apply tposr_eq_trans with (llift_rec 1 X n) ; auto with coc.
 
 
-assert (tposr_wf (llift_rec 1 A' n :: f)) by (apply wf_cons with (llift_rec 1 A' n) s ; eauto with coc).
-assert (tposr_wf (llift_rec 1 A0 n :: f)) by (apply wf_cons with (llift_rec 1 A0 n) s ; eauto with coc).
-apply tposr_coerce_prod with s ; auto with coc.
+apply tposr_coerce_prod with s ; eauto with coc ecoc.
+
 
 assert (tposr_wf (llift_rec 1 A' n :: f)) by (apply wf_cons with (llift_rec 1 A' n) s ; eauto with coc).
 assert (tposr_wf (llift_rec 1 A0 n :: f)) by (apply wf_cons with (llift_rec 1 A0 n) s ; eauto with coc).
